Interference.thy
@@ -25,18 +25,70 @@ definition inter\<^sub>\<alpha> :: "'b rpred \<Rightarrow> 'b rpred \<Rightarrow
                                   (\<exists>M'. R,G \<turnstile>\<^sub>A P {\<alpha>'} M' \<and> R,G \<turnstile>\<^sub>A M' {\<beta>} Q)"
 
 
-lemma guar_sub:
-  assumes "guar\<^sub>\<alpha> \<alpha> G" "G \<subseteq> G'"
-  shows "guar\<^sub>\<alpha> \<alpha> G'" using assms unfolding guar_def by auto
+text \<open>
+Independence of program c and instruction \<alpha> under environment R/G and memory model w,
+such that the early execution of \<alpha> cannot invalidate sequential reasoning.
+Define by recursively iterating over the program and capturing the forwarding throughout.\<close>
+fun inter\<^sub>c :: "('a,'b) wmm \<Rightarrow> 'b rpred \<Rightarrow> 'b rpred \<Rightarrow> ('a,'b) com \<Rightarrow> ('a,'b) basic \<Rightarrow> bool"
+  where 
+    "inter\<^sub>c w R G (Basic \<beta>) \<alpha> = (\<forall>\<alpha>'. w \<alpha>' \<beta> \<alpha> \<longrightarrow> inter\<^sub>\<alpha> R G \<alpha>' \<beta> \<alpha>)" |
+    "inter\<^sub>c w R G (c\<^sub>1 ;\<^sub>_ c\<^sub>2) \<alpha> = (\<forall>\<alpha>'. \<alpha>' < c\<^sub>2 <\<^sub>w \<alpha> \<longrightarrow> (inter\<^sub>c w R G c\<^sub>1 \<alpha>' \<and> inter\<^sub>c w R G c\<^sub>2 \<alpha>))" |
+    "inter\<^sub>c w R G (Nil) \<alpha> = True" | 
+    "inter\<^sub>c w R G _ \<alpha> = False"
+
+text \<open>
+Independence implications of the bookkeeping data structure collected 
+via the instrumented semantics.\<close> 
+fun inter :: "'b rpred \<Rightarrow> 'b rpred \<Rightarrow> ('a,'b) bookkeeping \<Rightarrow> bool"
+  where
+    "inter R G ((Reorder \<alpha>' w c)#r) = (inter\<^sub>c w R G c \<alpha>' \<and> inter R G r)" | 
+    "inter R G (Scope#r) = (inter (pushrelSame R) (pushrelAll G) r)" | 
+    "inter R G [] = True"
 
 
-lemma atomic_supG:
-  assumes "R,G \<turnstile>\<^sub>A M {\<alpha>} Q" "G \<subseteq> G'"
-  shows "R,G' \<turnstile>\<^sub>A M {\<alpha>} Q" using assms atomic_rule_def guar_sub by blast
 
-lemma atomic_subG:
-  assumes "R,G \<turnstile>\<^sub>A M {\<alpha>} Q" "guar\<^sub>\<alpha> \<alpha> G'"
-  shows "R,G' \<turnstile>\<^sub>A M {\<alpha>} Q" using assms atomic_rule_def by metis
+
+text \<open>Compute possible reorderings of the program using the instrumented semantics.\<close>
+inductive reorder_trace
+  where 
+    "reorder_trace [] c" |
+    "c \<leadsto> c' \<Longrightarrow> reorder_trace t c' \<Longrightarrow> reorder_trace t c" |
+    "c \<mapsto>[\<alpha>',r] c' \<Longrightarrow> reorder_trace t c' \<Longrightarrow> reorder_trace (r#t) c"
+
+text \<open>Ensure all reorderings enforce the necessary interference property\<close>
+definition rif
+  where "rif R G c \<equiv> \<forall>t. reorder_trace t c \<longrightarrow> (\<forall>r \<in> set t. inter R G r)"
+
+section \<open>Interference Properties\<close>
+
+text \<open>Interference check is preserved across a silent step\<close>
+lemma inter_silentI [intro]:
+  assumes "rif R G c" "c \<leadsto> c'"
+  shows "rif R G c'"
+  using assms by (auto simp: rif_def intro: reorder_trace.intros)
+
+text \<open>Interference check is preserved across an execution step and prevents interference\<close>
+lemma indep_stepI [intro]:
+  assumes "rif R G c" "c \<mapsto>[\<alpha>',r] c'"
+  shows "rif R G c' \<and> inter R G r"
+proof -
+  have "reorder_trace [r] c" using assms reorder_trace.intros by blast
+  hence "inter R G r" using assms by (auto simp: rif_def)
+  moreover have "rif R G c'"
+    using assms by (clarsimp simp: rif_def) (force intro: reorder_trace.intros(3))
+  ultimately show ?thesis by simp
+qed
+
+lemma inter_monoG:
+  assumes "G \<subseteq> G'" "inter R G r"
+  shows "inter R G' r" sorry
+
+end
+
+end
+
+
+(*
 
 lemma invarIQ:
   assumes "R,G \<turnstile>\<^sub>A P {\<alpha>} Q" "G \<subseteq> (I \<Zinj> I)" "P \<subseteq> I" "stable R I"
@@ -98,65 +150,4 @@ lemma interAtom2:
           "I \<subseteq> (vc \<beta>)" "I \<subseteq> (vc \<alpha>)" "I \<subseteq> Q"
   shows "inter\<^sub>\<alpha> R G \<alpha>' \<beta> \<alpha>" using assms interAtom inter\<^sub>\<alpha>_def sorry
 
-
-
-
-text \<open>
-Independence of program c and instruction \<alpha> under environment R/G and memory model w,
-such that the early execution of \<alpha> cannot invalidate sequential reasoning.
-Define by recursively iterating over the program and capturing the forwarding throughout.\<close>
-fun inter\<^sub>c :: "('a,'b) wmm \<Rightarrow> 'b rpred \<Rightarrow> 'b rpred \<Rightarrow> ('a,'b) com \<Rightarrow> ('a,'b) basic \<Rightarrow> bool"
-  where 
-    "inter\<^sub>c w R G (Basic \<beta>) \<alpha> = (\<forall>\<alpha>'. w \<alpha>' \<beta> \<alpha> \<longrightarrow> inter\<^sub>\<alpha> R G \<alpha>' \<beta> \<alpha>)" |
-    "inter\<^sub>c w R G (c\<^sub>1 ;\<^sub>_ c\<^sub>2) \<alpha> = (\<forall>\<alpha>'. \<alpha>' < c\<^sub>2 <\<^sub>w \<alpha> \<longrightarrow> (inter\<^sub>c w R G c\<^sub>1 \<alpha>' \<and> inter\<^sub>c w R G c\<^sub>2 \<alpha>))" |
-    "inter\<^sub>c w R G (Nil) \<alpha> = True" | 
-    "inter\<^sub>c w R G _ \<alpha> = False"
-
-text \<open>
-Independence implications of the bookkeeping data structure collected 
-via the instrumented semantics.\<close> 
-fun inter :: "'b rpred \<Rightarrow> 'b rpred \<Rightarrow> ('a,'b) bookkeeping \<Rightarrow> bool"
-  where
-    "inter R G ((Reorder \<alpha>' w c)#r) = (inter\<^sub>c w R G c \<alpha>' \<and> inter R G r)" | 
-    "inter R G (Scope#r) = (inter (pushrelSame R) (pushrelAll G) r)" | 
-    "inter R G [] = True"
-
-
-text \<open>Compute possible reorderings of the program using the instrumented semantics.\<close>
-inductive reorder_trace
-  where 
-    "reorder_trace [] c" |
-    "c \<leadsto> c' \<Longrightarrow> reorder_trace t c' \<Longrightarrow> reorder_trace t c" |
-    "c \<mapsto>[\<alpha>',r] c' \<Longrightarrow> reorder_trace t c' \<Longrightarrow> reorder_trace (r#t) c"
-
-text \<open>Ensure all reorderings enforce the necessary interference property\<close>
-definition rif
-  where "rif R G c \<equiv> \<forall>t. reorder_trace t c \<longrightarrow> (\<forall>r \<in> set t. inter R G r)"
-
-section \<open>Interference Properties\<close>
-
-text \<open>Interference check is preserved across a silent step\<close>
-lemma inter_silentI [intro]:
-  assumes "rif R G c" "c \<leadsto> c'"
-  shows "rif R G c'"
-  using assms by (auto simp: rif_def intro: reorder_trace.intros)
-
-text \<open>Interference check is preserved across an execution step and prevents interference\<close>
-lemma indep_stepI [intro]:
-  assumes "rif R G c" "c \<mapsto>[\<alpha>',r] c'"
-  shows "rif R G c' \<and> inter R G r"
-proof -
-  have "reorder_trace [r] c" using assms reorder_trace.intros by blast
-  hence "inter R G r" using assms by (auto simp: rif_def)
-  moreover have "rif R G c'"
-    using assms by (clarsimp simp: rif_def) (force intro: reorder_trace.intros(3))
-  ultimately show ?thesis by simp
-qed
-
-lemma inter_monoG:
-  assumes "G \<subseteq> G'" "inter R G r"
-  shows "inter R G' r" sorry
-
-end
-
-end
+*)
